update until Memory_Model.thy

logic/RT_Map.thy
@@ -13,31 +13,12 @@ begin
 definition
   partial_inj :: "('a \<Rightarrow> 'b option ) \<Rightarrow> bool"
 where
-  "partial_inj f \<equiv> \<forall>x. \<forall>y. if   x = y 
-                           then f x = f y
-                           else if f x = f y
-                                then f x = None \<and> f y = None
-                                else \<exists>a1 a2. a1 \<noteq> a2 \<and> f x = a1 \<and> f y = a2"
-
-lemma "partial_inj f = (\<forall>x y. x \<noteq> y \<longrightarrow> f x \<noteq> f y \<or> f x = None \<and> f y = None)"
-  by (auto simp add: partial_inj_def)
-
-(* update the logic semantics to assign the asids for the root *)
-
-(*  boot conditions *)
-
-
-lemma aval_state_rt_map_eq[simp]:
-  "(aval e (s\<lparr>root_map := root_map s(Addr r \<mapsto> a)\<rparr>) = Some v) = (aval e s = Some v)"
-  by (induct e arbitrary: v; clarsimp split: option.splits; fastforce)
-
+  "partial_inj f \<equiv>  (\<forall>x y. x \<noteq> y \<longrightarrow> f x \<noteq> f y \<or> f x = None \<and> f y = None)"
 
 
 lemma  rt_map_none_partial_inj:
   "(\<forall>rt. root_map s rt = None) \<Longrightarrow> partial_inj (root_map s)"
   by (clarsimp simp: partial_inj_def)
-
-
 
 lemma rt_map_update_none_partial:
   "\<Turnstile> \<lbrace> \<lambda>s. mode s = Kernel \<and>  aval rt s = Some v \<and> (\<forall>rt. root_map s rt = None)\<rbrace>
@@ -79,60 +60,40 @@ done
 
 
 
-definition
-  set_of_assigned_asids :: "rt_map_t \<Rightarrow> asid set"
-where
-  "set_of_assigned_asids rt_map \<equiv> {a. \<exists>x. rt_map x = Some a}" term "ran rtmap"
-
-(* have some lemmas about partial_injectivity *)
-
 lemma
-  "\<lbrakk>a1 \<in> set_of_assigned_asids rt_map\<rbrakk> \<Longrightarrow> \<exists>x. rt_map x = Some a1"
-  apply (clarsimp simp: set_of_assigned_asids_def)
+  "\<lbrakk>a1 \<in> ran rt_map\<rbrakk> \<Longrightarrow> \<exists>x. rt_map x = Some a1"
+  apply (clarsimp simp:  ran_def)
 done
 
 
 lemma part_inj_root_map_different_asids:
-  "\<lbrakk>a \<in> set_of_assigned_asids rt_map ; partial_inj rt_map\<rbrakk> \<Longrightarrow> \<exists>x. rt_map x = Some a \<and> (\<forall>y. x \<noteq> y \<longrightarrow> rt_map y \<noteq> Some a)"
-  apply (clarsimp simp: set_of_assigned_asids_def)
-  apply (rule_tac x = x in exI) 
-  apply simp
-  apply (rule allI)
-  apply (rule impI)
-  unfolding partial_inj_def
-  apply (erule_tac x = x in allE)
-  apply (erule_tac x = y in allE)
-  by auto
+  "\<lbrakk>a \<in> ran rt_map ; partial_inj rt_map\<rbrakk> \<Longrightarrow> \<exists>x. rt_map x = Some a \<and> (\<forall>y. x \<noteq> y \<longrightarrow> rt_map y \<noteq> Some a)"
+  apply (clarsimp simp: ran_def partial_inj_def)
+  by force
 
 
-definition  "asid_va_set (a::asid) \<equiv> (\<lambda>va::32 word. (a , va)) ` UNIV"   term "{a} \<times> UNIV" 
+definition "assigned_asid_va_map rt_map   \<equiv> \<Union>((\<lambda>x. {x} \<times> UNIV) ` ran rt_map)"
 
-definition "asids_va_set rt_map   \<equiv> \<Union>((\<lambda>x. asid_va_set x) ` set_of_assigned_asids rt_map)"
+definition "assigned_asids_consistent rt_map iset  \<equiv> assigned_asid_va_map rt_map \<inter> iset = {}"
+
+
+(*definition
+  set_of_assigned_asids :: "rt_map_t \<Rightarrow> asid set"
+where
+  "set_of_assigned_asids rt_map \<equiv> ran rt_map" *)    
+
                                                                          
-definition "assinged_asids_consistent rt_map iset  \<equiv> asids_va_set rt_map \<inter> iset = {}"
+(*definition  "asid_va_set (a::asid) \<equiv> {a} \<times> UNIV" *)
+
+(*definition "assinged_asids_consistent rt_map iset  \<equiv> asids_va_set rt_map \<inter> iset = {}"*)
 
 
-
-(*  trivial *)
+(* trivial *)
 lemma rt_map_update_boot_incon_set:
   "\<Turnstile> \<lbrace> \<lambda>s. mode s = Kernel \<and> (\<exists>v. aval rt s = Some v) \<and> incon_set s = {} \<and> (\<forall>rt. root_map s rt = None)\<rbrace>
-                UpdateRTMap rt a  \<lbrace>\<lambda>s. partial_inj (root_map s) \<and> asids_va_set (root_map s) \<inter> incon_set s = {} \<rbrace>"
+                UpdateRTMap rt a  \<lbrace>\<lambda>s. partial_inj (root_map s) \<and> assigned_asid_va_map  (root_map s) \<inter> incon_set s = {} \<rbrace>"
   apply vcg
   by (clarsimp simp: partial_inj_def)
-
-
-(*  trivial *)
-lemma rt_map_update_boot_incon_set:
-  "\<Turnstile> \<lbrace> \<lambda>s. mode s = Kernel \<and> (\<exists>v. aval rt s = Some v) \<and>  asids_va_set (root_map s) \<inter> incon_set s = {} \<and> (\<forall>rt. root_map s rt = None)\<rbrace>
-                UpdateRTMap rt a  \<lbrace>\<lambda>s. partial_inj (root_map s) \<and> asids_va_set (root_map s) \<inter> incon_set s = {} \<rbrace>"
-  apply vcg
-  apply (clarsimp simp: partial_inj_def asids_va_set_def set_of_assigned_asids_def asid_va_set_def)
-oops
-
-
-
-
-
 
 
 
