logic/Con_Set.thy
@@ -25,10 +25,6 @@ lemma flush_ASID_mem_write':
       ptable_lift_m (heap s) (root s) (mode s) (Addr vp) = Some pp \<rbrace>  Flush (flushASID a) ;; lval ::= rval \<lbrace>\<lambda>s. heap s pp = Some v \<rbrace>"
   by vcg
 
-lemma flush_va_mem_write':
-  "\<Turnstile> \<lbrace> \<lambda>s. aval lval s = Some vp \<and> aval rval s = Some v \<and> vp \<notin> SA  \<and> con_set SA s \<and> mode s = Kernel \<and> 
-     ptable_lift_m (heap s) (root s) (mode s) (Addr vp) = Some pp \<rbrace>  Flush (flushva (Addr vp)) ;; lval ::= rval \<lbrace>\<lambda>s. heap s pp = Some v \<rbrace>"
-  by vcg
 
 lemma flush_ASID_va_mem_write':
   "\<Turnstile> \<lbrace> \<lambda>s. aval lval s = Some vp \<and> aval rval s = Some v \<and> asid s = a \<and> vp \<notin> SA \<and> con_set SA s \<and> mode s = Kernel \<and> 
