logic/VCG_Check.thy
@@ -8,20 +8,6 @@ begin
 
 (* theorems for the checking the correctness of vcg *)
 
-(* simplification theorems for the aval *)
-
-lemma aval_state_incon_eq[simp]:
-  "(aval e (s\<lparr>incon_set := iset\<rparr>) = Some v) = (aval e s = Some v)"
-  by (induct e arbitrary: v; clarsimp split: option.splits; fastforce)
-
-lemma aval_state_mode_eq[simp]:
-  "(aval e (s\<lparr>mode := m\<rparr>) = Some v) = (aval e s = Some v)"
-  by (induct e arbitrary: v; clarsimp split: option.splits; fastforce)
-
-lemma aval_state_incon_mode_eq[simp]:
-  "(aval e (s\<lparr>incon_set := iset, mode := m\<rparr>) = Some v) = (aval e s = Some v)"
-  by clarsimp
-
 
 
 lemma  write_consistent_defined_address:
@@ -41,12 +27,6 @@ lemma flush_ASID_mem_write:
   "\<Turnstile> \<lbrace> \<lambda>s. aval lval s = Some vp \<and> aval rval s = Some v \<and> asid s = a \<and>  (a, vp) \<in> incon_set s \<and> mode s = Kernel \<and> 
       ptable_lift_m (heap s) (root s) (mode s) (Addr vp) = Some pp \<rbrace>  Flush (flushASID a) ;; lval ::= rval \<lbrace>\<lambda>s. heap s pp = Some v \<rbrace>"
     by vcg
-
-
-lemma flush_va_mem_write:
-  "\<Turnstile> \<lbrace> \<lambda>s. aval lval s = Some vp \<and> aval rval s = Some v \<and> (asid s, vp) \<in> incon_set s \<and> mode s = Kernel \<and> 
-      ptable_lift_m (heap s) (root s) (mode s) (Addr vp) = Some pp \<rbrace>  Flush (flushva (Addr vp)) ;; lval ::= rval \<lbrace>\<lambda>s. heap s pp = Some v \<rbrace>"
-  by vcg
 
 
 lemma flush_ASID_va_mem_write:
